ImplSync progress

disk-betree/ImplSync.i.dfy
@@ -1,12 +1,13 @@
 include "Impl.i.dfy"
 include "ImplIO.i.dfy"
 include "ImplSplit.i.dfy"
-//include "ImplFlush.i.dfy"
+include "ImplFlush.i.dfy"
 include "ImplFlushRootBucket.i.dfy"
 include "ImplGrow.i.dfy"
 include "ImplDealloc.i.dfy"
 include "ImplLeaf.i.dfy"
 include "ImplModelSync.i.dfy"
+include "ImplModelCache.i.dfy"
 include "MainDiskIOHandler.s.dfy"
 include "../lib/Option.s.dfy"
 include "../lib/Sets.i.dfy"
@@ -18,12 +19,15 @@ module ImplSync {
   import opened ImplIO
   import opened ImplSplit
   import opened ImplCache
-  //import opened ImplFlush
+  import opened ImplFlush
   import opened ImplFlushRootBucket
   import opened ImplDealloc
   import opened ImplGrow
   import opened ImplLeaf
   import ImplModelSync
+  import ImplModelCache
+  import ImplModelDealloc
+  import opened ImplState
 
   import opened Options
   import opened Maps
@@ -39,17 +43,20 @@ module ImplSync {
   requires Inv(k, s)
   requires s.Ready?
   requires ref in s.cache
-  requires parentref in IS.IIndirectionTable(s.ephemeralIndirectionTable)
-  requires ref in IS.IIndirectionTable(s.ephemeralIndirectionTable)[parentref].1
+  requires parentref in IIndirectionTable(s.ephemeralIndirectionTable)
+  requires ref in IIndirectionTable(s.ephemeralIndirectionTable)[parentref].1
   requires s.rootBucket == TTT.EmptyTree // FIXME we don't actually need this I think
   requires ref != BT.G.Root()
   requires io.initialized()
   modifies io
-  ensures IS.WVars(s')
+  ensures WVars(s')
+  ensures (IVars(s'), IIO(io)) == ImplModelSync.fixBigNode(Ic(k), old(IVars(s)), old(IIO(io)), ref, parentref)
   // NOALIAS statically enforced no-aliasing would probably help here
   ensures forall r | r in s.ephemeralIndirectionTable.Repr :: fresh(r) || r in old(s.ephemeralIndirectionTable.Repr)
   modifies s.ephemeralIndirectionTable.Repr
   {
+    ImplModelSync.reveal_fixBigNode();
+
     if (ref !in s.cache) {
       s' := PageInReq(k, s, io, ref);
       return;
@@ -67,9 +74,13 @@ module ImplSync {
       }
     }
 
+    ImplModelCache.lemmaGraphChildInGraph(Ic(k), IVars(s), parentref, ref);
+    assert IIndirectionTable(s.ephemeralIndirectionTable)[parentref].1
+        == IM.IIndirectionTable(IIndirectionTable(s.ephemeralIndirectionTable)).graph[parentref];
+
     var node := s.cache[ref];
 
-    var i := getUncappedBucket(node.buckets, 0);
+    var i := ImplModelSync.getUncappedBucket(node.buckets, 0);
     if i.Some? {
       if (node.children.Some?) {
         // internal node case: flush
@@ -77,21 +88,22 @@ module ImplSync {
         return;
       } else {
         // leaf case
-        s' := repivotLeaf(k, s, io, ref, i.value, node);
+        s' := repivotLeaf(k, s, ref, i.value, node);
         return;
       }
-    } else if |node.buckets| > Marshalling.CapNumBuckets() as int {
+    } else if |node.buckets| > IMM.CapNumBuckets() as int {
       if (parentref !in s.cache) {
+        ImplModelSync.lemmaRefHasLoc(Ic(k), IVars(s), parentref);
         s' := PageInReq(k, s, io, parentref);
         return;
       }
 
       var parent := s.cache[parentref];
 
-      assert ref in BT.G.Successors(IS.INode(parent));
+      assert ref in BT.G.Successors(IM.INode(parent));
       var j := SeqIndex(parent.children.value, ref);
 
-      s' := doSplit(k, s, io, parentref, ref, j.value);
+      s' := doSplit(k, s, parentref, ref, j.value);
       return;
     } else {
       s' := s;
@@ -100,32 +112,31 @@ module ImplSync {
     }
   }
 
-  /*
-  method AssignRefToLBA(table: IS.MutIndirectionTable, ref: IS.Reference, loc: BC.Location)
+  method AssignRefToLoc(table: MutIndirectionTable, ref: Reference, loc: BC.Location)
   requires table.Inv()
   ensures table.Inv()
-  ensures IS.IIndirectionTable(table) == old(BC.assignRefToLocation(IS.IIndirectionTable(table), ref, loc))
   // NOALIAS statically enforced no-aliasing would probably help here
   ensures forall r | r in table.Repr :: fresh(r) || r in old(table.Repr)
   modifies table.Repr
+  ensures table.Contents == ImplModelSync.AssignRefToLoc(old(table.Contents), ref, loc)
   {
+    ImplModelSync.reveal_AssignRefToLoc();
     var locGraph := table.Remove(ref);
     if locGraph.Some? {
       var (_, graph) := locGraph.value;
       assume table.Count as nat < 0x10000000000000000 / 8;
       var _ := table.Insert(ref, (Some(loc), graph));
     }
-    assert IS.IIndirectionTable(table) ==
-        old(BC.assignRefToLocation(IS.IIndirectionTable(table), ref, loc));
+    //assert IIndirectionTable(table) ==
+    //    old(BC.assignRefToLocation(IIndirectionTable(table), ref, loc));
   }
 
-  method FindUncappedNodeInCache(s: ImplVariables) returns (ref: Option<IS.Reference>)
-  requires IS.WFVars(s)
+  method FindUncappedNodeInCache(s: ImplVariables) returns (ref: Option<Reference>)
+  requires WFVars(s)
   requires s.Ready?
-  ensures ref.Some? ==> ref.value in IS.IIndirectionTable(s.ephemeralIndirectionTable).graph
-  ensures ref.Some? ==> ref.value in s.cache && !Marshalling.CappedNode(s.cache[ref.value])
-  ensures ref.None? ==> forall r | r in IS.IIndirectionTable(s.ephemeralIndirectionTable).graph :: r !in s.cache || Marshalling.CappedNode(s.cache[r])
+  ensures ref == ImplModelSync.FindUncappedNodeInCache(IVars(s))
   {
+    assume false;
     // TODO once we have an lba freelist, rewrite this to avoid extracting a `map` from `s.ephemeralIndirectionTable`
     var ephemeralTable := s.ephemeralIndirectionTable.ToMap();
     var ephemeralRefs := SetToSeq(ephemeralTable.Keys);
@@ -136,28 +147,26 @@ module ImplSync {
     while i as int < |ephemeralRefs|
     invariant i as int <= |ephemeralRefs|
     invariant forall k : nat | k < i as nat :: (
-        && ephemeralRefs[k] in IS.IIndirectionTable(s.ephemeralIndirectionTable).graph
-        && (ephemeralRefs[k] !in s.cache || Marshalling.CappedNode(s.cache[ephemeralRefs[k]])))
+        && ephemeralRefs[k] in IM.IIndirectionTable(IIndirectionTable(s.ephemeralIndirectionTable)).graph
+        && (ephemeralRefs[k] !in s.cache || IMM.CappedNode(s.cache[ephemeralRefs[k]])))
     {
       var ref := ephemeralRefs[i];
-      if ref in s.cache && !Marshalling.CappedNode(s.cache[ref]) {
+      if ref in s.cache && !IMM.CappedNode(s.cache[ref]) {
         return Some(ref);
       }
       i := i + 1;
     }
-    assert forall r | r in IS.IIndirectionTable(s.ephemeralIndirectionTable).graph :: r !in s.cache || Marshalling.CappedNode(s.cache[r]);
+    assert forall r | r in IM.IIndirectionTable(IIndirectionTable(s.ephemeralIndirectionTable)).graph :: r !in s.cache || IMM.CappedNode(s.cache[r]);
     return None;
   }
 
-  method FindRefInFrozenWithNoLba(s: ImplVariables) returns (ref: Option<IS.Reference>)
-  requires IS.WFVars(s)
+  method FindRefInFrozenWithNoLoc(s: ImplVariables) returns (ref: Option<Reference>)
+  requires WFVars(s)
   requires s.Ready?
   requires s.frozenIndirectionTable.Some?
-  ensures ref.Some? ==> ref.value in IS.IIndirectionTable(s.frozenIndirectionTable.value).graph 
-  ensures ref.Some? ==> ref.value !in IS.IIndirectionTable(s.frozenIndirectionTable.value).locs
-  ensures ref.None? ==> forall r | r in IS.IIndirectionTable(s.frozenIndirectionTable.value).graph
-      :: r in IS.IIndirectionTable(s.frozenIndirectionTable.value).locs
+  ensures ref == ImplModelSync.FindRefInFrozenWithNoLoc(IVars(s))
   {
+    assume false;
     // TODO once we have an lba freelist, rewrite this to avoid extracting a `map` from `s.ephemeralIndirectionTable`
     var frozenTable := s.frozenIndirectionTable.value.ToMap();
     var frozenRefs := SetToSeq(frozenTable.Keys);
@@ -168,8 +177,8 @@ module ImplSync {
     while i as int < |frozenRefs|
     invariant i as int <= |frozenRefs|
     invariant forall k : nat | k < i as nat :: (
-        && frozenRefs[k] in IS.IIndirectionTable(s.frozenIndirectionTable.value).graph
-        && frozenRefs[k] in IS.IIndirectionTable(s.frozenIndirectionTable.value).locs)
+        && frozenRefs[k] in IM.IIndirectionTable(IIndirectionTable(s.frozenIndirectionTable.value)).graph
+        && frozenRefs[k] in IM.IIndirectionTable(IIndirectionTable(s.frozenIndirectionTable.value)).locs)
     {
       var ref := frozenRefs[i];
       var lbaGraph := s.frozenIndirectionTable.value.Get(ref);
@@ -180,26 +189,24 @@ module ImplSync {
       }
       i := i + 1;
     }
-    assert forall r | r in IS.IIndirectionTable(s.frozenIndirectionTable.value).graph
-        :: r in IS.IIndirectionTable(s.frozenIndirectionTable.value).locs;
+    assert forall r | r in IM.IIndirectionTable(IIndirectionTable(s.frozenIndirectionTable.value)).graph
+        :: r in IM.IIndirectionTable(IIndirectionTable(s.frozenIndirectionTable.value)).locs;
     return None;
   }
 
-  method FindRefNotPointingToRefInEphemeral(s: ImplVariables, ref: IS.Reference) returns (result: IS.Reference)
-  requires IS.WFVars(s)
+  method FindParentRef(s: ImplVariables, ref: Reference) returns (result: Reference)
+  requires WFVars(s)
   requires s.Ready?
-  requires exists r :: r in IS.IIndirectionTable(s.ephemeralIndirectionTable).graph && 
-      ref in IS.IIndirectionTable(s.ephemeralIndirectionTable).graph[r]
-  ensures result in IS.IIndirectionTable(s.ephemeralIndirectionTable).graph && 
-      ref in IS.IIndirectionTable(s.ephemeralIndirectionTable).graph[result]
+  ensures result == ImplModelSync.FindParentRef(IVars(s), ref)
   {
+    assume false;
     assert s.ephemeralIndirectionTable.Inv();
     var ephemeralTable := s.ephemeralIndirectionTable.ToMap();
 
     var ephemeralRefs := SetToSeq(ephemeralTable.Keys);
     assert forall k | k in ephemeralRefs :: k in ephemeralTable;
 
-    assert forall k | k in ephemeralRefs :: k in IS.IIndirectionTable(s.ephemeralIndirectionTable).graph; // TODO
+    assert forall k | k in ephemeralRefs :: k in IM.IIndirectionTable(IIndirectionTable(s.ephemeralIndirectionTable)).graph; // TODO
 
     // TODO how do we deal with this?
     assume |ephemeralRefs| < 0x1_0000_0000_0000_0000;
@@ -208,19 +215,19 @@ module ImplSync {
     while i as nat < |ephemeralRefs|
     invariant i as nat <= |ephemeralRefs|
     invariant forall k : nat | k < i as nat :: (
-        || ephemeralRefs[k] !in IS.IIndirectionTable(s.ephemeralIndirectionTable).graph
-        || ref !in IS.IIndirectionTable(s.ephemeralIndirectionTable).graph[ephemeralRefs[k]])
+        || ephemeralRefs[k] !in IM.IIndirectionTable(IIndirectionTable(s.ephemeralIndirectionTable)).graph
+        || ref !in IM.IIndirectionTable(IIndirectionTable(s.ephemeralIndirectionTable)).graph[ephemeralRefs[k]])
     {
       var eRef := ephemeralRefs[i];
-      assert eRef in IS.IIndirectionTable(s.ephemeralIndirectionTable).graph;
+      assert eRef in IM.IIndirectionTable(IIndirectionTable(s.ephemeralIndirectionTable)).graph;
 
       var lbaGraph := s.ephemeralIndirectionTable.Get(eRef);
       assert lbaGraph.Some?;
 
       var (_, graph) := lbaGraph.value;
       if ref in graph {
-        assert eRef in IS.IIndirectionTable(s.ephemeralIndirectionTable).graph && 
-            ref in IS.IIndirectionTable(s.ephemeralIndirectionTable).graph[eRef];
+        assert eRef in IM.IIndirectionTable(IIndirectionTable(s.ephemeralIndirectionTable)).graph && 
+            ref in IM.IIndirectionTable(IIndirectionTable(s.ephemeralIndirectionTable)).graph[eRef];
         return eRef;
       }
 
@@ -234,14 +241,13 @@ module ImplSync {
   returns (s': ImplVariables)
   requires io.initialized()
   modifies io
-  requires IS.WFVars(s)
-  requires BBC.Inv(k, IS.IVars(s))
+  requires Inv(k, s)
   requires s.Ready?
   requires s.outstandingIndirectionTableWrite.None?
   requires s.rootBucket == TTT.EmptyTree
   requires s.frozenIndirectionTable.None?
-  ensures IS.WFVars(s')
-  ensures ImplADM.M.Next(Ik(k), old(IS.IVars(s)), IS.IVars(s'), UI.NoOp, io.diskOp())
+  ensures WVars(s')
+  ensures (IVars(s'), IIO(io)) == ImplModelSync.syncNotFrozen(Ic(k), old(IVars(s)), old(IIO(io)))
   // NOALIAS statically enforced no-aliasing would probably help here
   ensures s.Ready? ==> forall r | r in s.ephemeralIndirectionTable.Repr :: fresh(r) || r in old(s.ephemeralIndirectionTable.Repr)
   modifies if s.Ready? then s.ephemeralIndirectionTable.Repr else {}
@@ -249,127 +255,101 @@ module ImplSync {
     var ephemeralTable := s.ephemeralIndirectionTable.ToMap();
     var ephemeralGraph := map k | k in ephemeralTable :: ephemeralTable[k].1;
     var foundDeallocable := FindDeallocable(s);
+    ImplModelDealloc.FindDeallocableCorrect(IVars(s));
     if foundDeallocable.Some? {
       s' := Dealloc(k, s, io, foundDeallocable.value);
       return;
     }
     var foundUncapped := FindUncappedNodeInCache(s);
+    ImplModelSync.FindUncappedNodeInCacheCorrect(IVars(s));
     if foundUncapped.Some? {
       var ref := foundUncapped.value;
-      assert ref in IS.IIndirectionTable(s.ephemeralIndirectionTable).graph;
-      assert ref in s.cache && !Marshalling.CappedNode(s.cache[foundUncapped.value]);
       if (ref == BT.G.Root()) {
         s' := fixBigRoot(k, s, io);
         return;
       } else {
-        assert !deallocable(s, ref);
-        assert !(forall r | r in IS.IIndirectionTable(s.ephemeralIndirectionTable).graph ::
-            ref !in IS.IIndirectionTable(s.ephemeralIndirectionTable).graph[r]);
-        assert !(forall r :: r in IS.IIndirectionTable(s.ephemeralIndirectionTable).graph ==>
-            ref !in IS.IIndirectionTable(s.ephemeralIndirectionTable).graph[r]);
-        assert (exists r :: !(r in IS.IIndirectionTable(s.ephemeralIndirectionTable).graph ==>
-            ref !in IS.IIndirectionTable(s.ephemeralIndirectionTable).graph[r]));
-        var r := FindRefNotPointingToRefInEphemeral(s, ref);
-        assert !(r in IS.IIndirectionTable(s.ephemeralIndirectionTable).graph ==>
-            ref !in IS.IIndirectionTable(s.ephemeralIndirectionTable).graph[r]);
+        var r := FindParentRef(s, ref);
+        ImplModelSync.FindParentRefCorrect(IVars(s), ref);
+
         s' := fixBigNode(k, s, io, ref, r);
         return;
       }
     } else {
       var clonedEphemeralIndirectionTable := s.ephemeralIndirectionTable.Clone();
-      assert IS.IIndirectionTable(clonedEphemeralIndirectionTable) == IS.IIndirectionTable(s.ephemeralIndirectionTable); // observe
 
       s' := s
           .(frozenIndirectionTable := Some(clonedEphemeralIndirectionTable))
           .(syncReqs := BC.syncReqs3to2(s.syncReqs));
 
-      assert BC.Freeze(Ik(k), old(IS.IVars(s)), IS.IVars(s'), ImplADM.M.IDiskOp(io.diskOp()));
-      assert BBC.BlockCacheMove(Ik(k), old(IS.IVars(s)), IS.IVars(s'), UI.NoOp, ImplADM.M.IDiskOp(io.diskOp()), BC.FreezeStep);
-      assert stepsBC(k, old(IS.IVars(s)), IS.IVars(s'), UI.NoOp, io, BC.FreezeStep);
       return;
     }
   }
 
-  method {:fuel BC.GraphClosed,0} syncFoundInFrozen(k: ImplConstants, s: ImplVariables, io: DiskIOHandler, ref: IS.Reference)
+  method {:fuel BC.GraphClosed,0} syncFoundInFrozen(k: ImplConstants, s: ImplVariables, io: DiskIOHandler, ref: Reference)
   returns (s': ImplVariables)
   requires io.initialized()
   modifies io
-  requires IS.WFVars(s)
-  requires BBC.Inv(k, IS.IVars(s))
+  requires Inv(k, s)
   requires s.Ready?
   requires s.outstandingIndirectionTableWrite.None?
   requires s.rootBucket == TTT.EmptyTree
   requires s.frozenIndirectionTable.Some?
-  requires ref in IS.IIndirectionTable(s.frozenIndirectionTable.value).graph 
-  requires ref !in IS.IIndirectionTable(s.frozenIndirectionTable.value).locs
-  ensures IS.WFVars(s')
-  ensures ImplADM.M.Next(Ik(k), old(IS.IVars(s)), IS.IVars(s'), UI.NoOp, io.diskOp())
+  requires ref in s.frozenIndirectionTable.value.Contents
+  requires s.frozenIndirectionTable.value.Contents[ref].0.None?
+  ensures WFVars(s')
+  ensures ImplModelSync.syncFoundInFrozen(Ic(k), old(IVars(s)), old(IIO(io)), ref, IVars(s'), IIO(io))
   // NOALIAS statically enforced no-aliasing would probably help here
   ensures s.Ready? ==> forall r | r in s.ephemeralIndirectionTable.Repr :: fresh(r) || r in old(s.ephemeralIndirectionTable.Repr)
   modifies if s.Ready? then s.ephemeralIndirectionTable.Repr else {}
   modifies if s.Ready? then s.frozenIndirectionTable.value.Repr else {}
   {
-    assert ref in IS.IIndirectionTable(s.frozenIndirectionTable.value).graph;
-    assert ref !in IS.IIndirectionTable(s.frozenIndirectionTable.value).locs;
+    assert ref in IM.IIndirectionTable(IIndirectionTable(s.frozenIndirectionTable.value)).graph;
+    assert ref !in IM.IIndirectionTable(IIndirectionTable(s.frozenIndirectionTable.value)).locs;
 
-    if (!Marshalling.CappedNode(s.cache[ref])) {
+    if (!IMM.CappedNode(s.cache[ref])) {
       // TODO we should be able to prove this is impossible by adding an invariant
       // about frozenIndirectionTable (that is, we should never be freezing a table
       // with too-big nodes in it)
       s' := s;
-      assert noop(k, old(IS.IVars(s)), IS.IVars(s'));
       print "sync: giving up; frozen table has big node rip (TODO we should prove this case impossible)\n";
       return;
     }
 
     var ephemeralRef := s.ephemeralIndirectionTable.Get(ref);
     if ephemeralRef.Some? && ephemeralRef.value.0.Some? {
-      assert ref in IS.IIndirectionTable(s.ephemeralIndirectionTable).locs;
       // TODO we should be able to prove this is impossible as well
       s' := s;
-      assert noop(k, old(IS.IVars(s)), IS.IVars(s'));
       print "sync: giving up; ref already in ephemeralIndirectionTable.locs but not frozen";
       return;
     }
 
-    assert ref !in IS.IIndirectionTable(s.ephemeralIndirectionTable).locs;
+    var id, loc := FindLocationAndRequestWrite(io, s, SectorBlock(s.cache[ref]));
 
-    INodeRootEqINodeForEmptyRootBucket(s.cache[ref]);
-    var id, loc := FindLocationAndRequestWrite(s, io, IS.SectorBlock(s.cache[ref]));
     if (id.Some?) {
-      assert loc.value == ImplADM.M.IDiskOp(io.diskOp()).reqWrite.loc;
-      /* (doc) assert reqWriteLoc.addr != BC.IndirectionTableLBA(); */
-      /* (doc) assert BC.ValidAllocation(old(IS.IVars(s)), loc.value); */
-
-      AssignRefToLBA(s.ephemeralIndirectionTable, ref, loc.value);
-      assert IS.IIndirectionTable(s.ephemeralIndirectionTable) ==
-        BC.assignRefToLocation(IS.IIndirectionTable(s.ephemeralIndirectionTable), ref, loc.value);
-      AssignRefToLBA(s.frozenIndirectionTable.value, ref, loc.value);
-      assert IS.IIndirectionTable(s.frozenIndirectionTable.value) ==
-        BC.assignRefToLocation(IS.IIndirectionTable(s.frozenIndirectionTable.value), ref, loc.value);
+      AssignRefToLoc(s.ephemeralIndirectionTable, ref, loc.value);
+      AssignRefToLoc(s.frozenIndirectionTable.value, ref, loc.value);
       s' := s
         .(outstandingBlockWrites := s.outstandingBlockWrites[id.value := BC.OutstandingWrite(ref, loc.value)]);
 
-      assert BC.ValidLocationForNode(ImplADM.M.IDiskOp(io.diskOp()).reqWrite.loc);
-      assert BC.WriteBackReq(Ik(k), old(IS.IVars(s)), IS.IVars(s'), ImplADM.M.IDiskOp(io.diskOp()), ref);
-      assert stepsBC(k, old(IS.IVars(s)), IS.IVars(s'), UI.NoOp, io, BC.WriteBackReqStep(ref));
-      return;
+      assert id == Some(io.diskOp().id);
+      ImplModelSync.reveal_AssignRefToLoc();
+      assert loc == s'.frozenIndirectionTable.value.Contents[ref].0;
     } else {
       s' := s;
-      assert noop(k, old(IS.IVars(s)), IS.IVars(s'));
       print "sync: giving up; write req failed\n";
-      return;
     }
   }
+
+  /*
 
   method {:fuel BC.GraphClosed,0} sync(k: ImplConstants, s: ImplVariables, io: DiskIOHandler)
   returns (s': ImplVariables)
   requires io.initialized()
   modifies io
-  requires IS.WFVars(s)
-  requires BBC.Inv(k, IS.IVars(s))
-  ensures IS.WFVars(s')
-  ensures ImplADM.M.Next(Ik(k), old(IS.IVars(s)), IS.IVars(s'), UI.NoOp, io.diskOp())
+  requires WFVars(s)
+  requires BBC.Inv(k, IVars(s))
+  ensures WFVars(s')
+  ensures ImplADM.M.Next(Ik(k), old(IVars(s)), IVars(s'), UI.NoOp, io.diskOp())
   // NOALIAS statically enforced no-aliasing would probably help here
   ensures s.Ready? ==> forall r | r in s.ephemeralIndirectionTable.Repr :: fresh(r) || r in old(s.ephemeralIndirectionTable.Repr)
   modifies if s.Ready? then s.ephemeralIndirectionTable.Repr else {}
@@ -383,7 +363,7 @@ module ImplSync {
 
     if (s.outstandingIndirectionTableWrite.Some?) {
       s' := s;
-      assert noop(k, old(IS.IVars(s)), IS.IVars(s'));
+      assert noop(k, old(IVars(s)), IVars(s'));
       print "sync: giving up; frozen table is currently being written\n";
       return;
     }
@@ -412,20 +392,20 @@ module ImplSync {
       return;
     } else if (s.outstandingBlockWrites != map[]) {
       s' := s;
-      assert noop(k, old(IS.IVars(s)), IS.IVars(s'));
+      assert noop(k, old(IVars(s)), IVars(s'));
       print "sync: giving up; blocks are still being written\n";
       return;
     } else {
       LBAType.reveal_ValidAddr();
-      var id := RequestWrite(io, BC.IndirectionTableLocation(), IS.SectorIndirectionTable(s.frozenIndirectionTable.value));
+      var id := RequestWrite(io, BC.IndirectionTableLocation(), SectorIndirectionTable(s.frozenIndirectionTable.value));
       if (id.Some?) {
         s' := s.(outstandingIndirectionTableWrite := id);
-        assert BC.WriteBackIndirectionTableReq(Ik(k), old(IS.IVars(s)), IS.IVars(s'), ImplADM.M.IDiskOp(io.diskOp()));
-        assert stepsBC(k, old(IS.IVars(s)), IS.IVars(s'), UI.NoOp, io, BC.WriteBackIndirectionTableReqStep);
+        assert BC.WriteBackIndirectionTableReq(Ik(k), old(IVars(s)), IVars(s'), ImplADM.M.IDiskOp(io.diskOp()));
+        assert stepsBC(k, old(IVars(s)), IVars(s'), UI.NoOp, io, BC.WriteBackIndirectionTableReqStep);
         return;
       } else {
         s' := s;
-        assert noop(k, old(IS.IVars(s)), IS.IVars(s'));
+        assert noop(k, old(IVars(s)), IVars(s'));
         print "sync: giving up; write back indirection table failed (no id)\n";
         return;
       }
@@ -449,14 +429,14 @@ module ImplSync {
   method pushSync(k: ImplConstants, s: ImplVariables, io: DiskIOHandler)
   returns (s': ImplVariables, id: int)
   requires io.initialized()
-  requires IS.WFVars(s)
-  requires BBC.Inv(k, IS.IVars(s))
-  ensures IS.WFVars(s')
-  ensures ImplADM.M.Next(Ik(k), old(IS.IVars(s)), IS.IVars(s'), UI.PushSyncOp(id), io.diskOp())
+  requires WFVars(s)
+  requires BBC.Inv(k, IVars(s))
+  ensures WFVars(s')
+  ensures ImplADM.M.Next(Ik(k), old(IVars(s)), IVars(s'), UI.PushSyncOp(id), io.diskOp())
   {
     id := freeId(s.syncReqs);
     s' := s.(syncReqs := s.syncReqs[id := BC.State3]);
-    assert stepsBC(k, IS.IVars(s), IS.IVars(s'), UI.PushSyncOp(id), io, BC.PushSyncReqStep(id));
+    assert stepsBC(k, IVars(s), IVars(s'), UI.PushSyncOp(id), io, BC.PushSyncReqStep(id));
   }
 
   // == popSync ==
@@ -464,11 +444,11 @@ module ImplSync {
   method popSync(k: ImplConstants, s: ImplVariables, io: DiskIOHandler, id: int)
   returns (s': ImplVariables, success: bool)
   requires io.initialized()
-  requires IS.WFVars(s)
-  requires BBC.Inv(k, IS.IVars(s))
+  requires WFVars(s)
+  requires BBC.Inv(k, IVars(s))
   modifies io
-  ensures IS.WFVars(s')
-  ensures ImplADM.M.Next(Ik(k), old(IS.IVars(s)), IS.IVars(s'), if success then UI.PopSyncOp(id) else UI.NoOp, io.diskOp())
+  ensures WFVars(s')
+  ensures ImplADM.M.Next(Ik(k), old(IVars(s)), IVars(s'), if success then UI.PopSyncOp(id) else UI.NoOp, io.diskOp())
   // NOALIAS statically enforced no-aliasing would probably help here
   ensures s.Ready? ==> forall r | r in s.ephemeralIndirectionTable.Repr :: fresh(r) || r in old(s.ephemeralIndirectionTable.Repr)
   modifies if s.Ready? then s.ephemeralIndirectionTable.Repr else {}
@@ -477,7 +457,7 @@ module ImplSync {
     if (id in s.syncReqs && s.syncReqs[id] == BC.State1) {
       success := true;
       s' := s.(syncReqs := MapRemove1(s.syncReqs, id));
-      assert stepsBC(k, IS.IVars(s), IS.IVars(s'), UI.PopSyncOp(id), io, BC.PopSyncReqStep(id));
+      assert stepsBC(k, IVars(s), IVars(s'), UI.PopSyncOp(id), io, BC.PopSyncReqStep(id));
     } else {
       success := false;
       s' := sync(k, s, io);
