disk-betree/ImplIO.i.dfy
@@ -108,6 +108,8 @@ module ImplIO {
   requires io.initialized()
   modifies io
   ensures ImplModelIO.FindLocationAndRequestWrite(old(IIO(io)), IS.IVars(s), ISector(sector), id, loc, IIO(io))
+  ensures id.Some? ==> loc.Some?
+  ensures id.None? ==> IIO(io) == old(IIO(io))
   {
     ImplModelIO.reveal_FindLocationAndRequestWrite();
 
